Move natural number development to separate file; add <= treatment.

examples/set-theory/vbg/vbgsetScript.sml
@@ -30,13 +30,14 @@ val SPEC0 = new_specification(
   "SPEC0",
   ["SPEC0"],
   CONV_RULE SKOLEM_CONV SPECIFICATION);
+val _ = export_rewrites ["SPEC0"]
 
 val EMPTY_def = Define`EMPTY = SPEC0 (λx. F)`
 
 val NOT_IN_EMPTY = store_thm(
   "NOT_IN_EMPTY",
   ``x ∉ {}``,
-  SRW_TAC [][EMPTY_def, SPEC0]);
+  SRW_TAC [][EMPTY_def]);
 val _ = export_rewrites ["NOT_IN_EMPTY"]
 
 val EMPTY_UNIQUE = store_thm(
@@ -85,7 +86,7 @@ val Sets_def = Define`Sets = SPEC0 (λx. T)`
 val SET_Sets = store_thm(
   "SET_Sets",
   ``x ∈ Sets <=> SET x``,
-  SRW_TAC [][Sets_def, SPEC0]);
+  SRW_TAC [][Sets_def]);
 
 val SUBSET_Sets = store_thm(
   "SUBSET_Sets",
@@ -101,8 +102,8 @@ val RUS_def = Define`
 *)
 val RUSlemma =
 ``RUS ∈ RUS``
-    |> (SIMP_CONV (srw_ss()) [RUS_def, Once SPEC0] THENC
-        SIMP_CONV (srw_ss()) [GSYM RUS_def])
+    |> (SIMP_CONV bool_ss [RUS_def, Once SPEC0] THENC
+        SIMP_CONV bool_ss [GSYM RUS_def])
 
 val RUS_not_SET = store_thm(
   "RUS_not_SET",
@@ -113,7 +114,7 @@ val POW_def = Define`POW A = SPEC0 (λx. x ⊆ A)`
 val IN_POW = store_thm(
   "IN_POW",
   ``x ∈ POW A ⇔ SET x ∧ x ⊆ A``,
-  SRW_TAC [][POW_def, SPEC0]);
+  SRW_TAC [][POW_def]);
 val _ = export_rewrites ["IN_POW"]
 
 val POWERSET = new_axiom(
@@ -143,12 +144,12 @@ val SINGC_def = Define`
 val PCLASS_SINGC_EMPTY = store_thm(
   "PCLASS_SINGC_EMPTY",
   ``¬SET a ⇒ (SINGC a = {})``,
-  SRW_TAC [][SINGC_def, SPEC0, Once EXTENSION]);
+  SRW_TAC [][SINGC_def, Once EXTENSION]);
 
 val SET_IN_SINGC = store_thm(
   "SET_IN_SINGC",
   ``SET a ⇒ (x ∈ SINGC a ⇔ (x = a))``,
-  SRW_TAC [CONJ_ss][SINGC_def, SPEC0]);
+  SRW_TAC [CONJ_ss][SINGC_def]);
 
 val SINGC_11 = store_thm(
   "SINGC_11",
@@ -168,14 +169,14 @@ val SINGC_PAIRC = store_thm(
 val PCLASS_PAIRC_EMPTY = store_thm(
   "PCLASS_PAIRC_EMPTY",
   ``¬SET a ∧ ¬SET b ⇒ (PAIRC a b = {})``,
-  SRW_TAC [][PAIRC_def, Once EXTENSION, SPEC0] THEN
+  SRW_TAC [][PAIRC_def, Once EXTENSION] THEN
   Cases_on `x = a` THEN SRW_TAC [][] THEN
   Cases_on `x = b` THEN SRW_TAC [][]);
 
 val SET_IN_PAIRC = store_thm(
   "SET_IN_PAIRC",
   ``SET a ∧ SET b ⇒ (∀x. x ∈ PAIRC a b ⇔ (x = a) ∨ (x = b))``,
-  SRW_TAC [CONJ_ss, DNF_ss][PAIRC_def, SPEC0]);
+  SRW_TAC [CONJ_ss, DNF_ss][PAIRC_def]);
 
 val UNORDERED_PAIRS = new_axiom(
   "UNORDERED_PAIRS",
@@ -203,14 +204,14 @@ val UNION_def = Define`a ∪ b = SPEC0 (λx. x ∈ a ∨ x ∈ b)`
 val IN_UNION = store_thm(
   "IN_UNION",
   ``x ∈ A ∪ B ⇔ x ∈ A ∨ x ∈ B``,
-  SRW_TAC [][UNION_def, SPEC0] THEN METIS_TAC [SET_def]);
+  SRW_TAC [][UNION_def] THEN METIS_TAC [SET_def]);
 val _ = export_rewrites ["IN_UNION"]
 
 val BIGUNION_def = Define`BIGUNION A = SPEC0 (λx. ∃y. y ∈ A ∧ x ∈ y)`
 val IN_BIGUNION = store_thm(
   "IN_BIGUNION",
   ``x ∈ BIGUNION A ⇔ ∃y. y ∈ A ∧ x ∈ y``,
-  SRW_TAC [][BIGUNION_def, SPEC0] THEN METIS_TAC [SET_def]);
+  SRW_TAC [][BIGUNION_def] THEN METIS_TAC [SET_def]);
 val _ = export_rewrites ["IN_BIGUNION"]
 
 val EMPTY_UNION = store_thm(
@@ -254,7 +255,7 @@ val INTER_def = Define`
 val IN_INTER = store_thm(
   "IN_INTER",
   ``e ∈ s1 ∩ s2 ⇔ SET e ∧ e ∈ s1 ∧ e ∈ s2``,
-  rw [INTER_def, SPEC0]);
+  rw [INTER_def]);
 val _ = export_rewrites ["IN_INTER"]
 
 val INTER_SET_CLOSED = store_thm(
@@ -377,12 +378,12 @@ val SET_OPAIR = store_thm(
   ``SET a ∧ SET b ⇒ SET (OPAIR a b)``,
   SRW_TAC [][OPAIR_def] THENL[
     SRW_TAC [][POPAIR_def] THEN MATCH_MP_TAC SUBSETS_ARE_SETS THEN
-    SRW_TAC [DNF_ss][SUBSET_def, SPEC0] THEN
+    SRW_TAC [DNF_ss][SUBSET_def] THEN
     Q.EXISTS_TAC `POW (POW (a ∪ {{}}))` THEN
     SRW_TAC [][POW_SET_CLOSED] THEN
     ASM_SIMP_TAC (srw_ss() ++ DNF_ss) [SUBSET_def],
     SRW_TAC [][POPAIR_def] THEN MATCH_MP_TAC SUBSETS_ARE_SETS THEN
-    SRW_TAC [DNF_ss][SUBSET_def, SPEC0] THEN
+    SRW_TAC [DNF_ss][SUBSET_def] THEN
     Q.EXISTS_TAC `POW (POW (b ∪ {{{}}}))` THEN
     SRW_TAC [][POW_SET_CLOSED] THEN
     ASM_SIMP_TAC (srw_ss() ++ DNF_ss) [SUBSET_def]
@@ -407,7 +408,7 @@ val OPAIR_11 = store_thm(
   "OPAIR_11",
   ``((OPAIR a b = OPAIR c d) ⇔ (a = c) ∧ (b = d))``,
   SRW_TAC [][Once EXTENSION, SimpLHS] THEN
-  SRW_TAC [][OPAIR_def, SPEC0] THEN
+  SRW_TAC [][OPAIR_def] THEN
   REVERSE EQ_TAC THEN1 SRW_TAC [][] THEN
   REPEAT STRIP_TAC THENL [
     SIMP_TAC (srw_ss()) [EXTENSION, EQ_IMP_THM] THEN
@@ -476,168 +477,38 @@ val apply_def = new_specification("apply_def",
                    RES_TAC THEN FULL_SIMP_TAC (srw_ss()) [OPAIR_11])
 *)
 
-val vSUC_def = Define`vSUC x = x ∪ {x}`
-
-val fromNat_def = Define`
-  (fromNat 0 = {}) ∧
-  (fromNat (SUC n) = vSUC (fromNat n))
-`;
-val _ = add_numeral_form(#"v", SOME "fromNat")
-
-val inductive_def = Define`
-  inductive A ⇔ SET A ∧ {} ∈ A ∧ ∀x. x ∈ A ⇒ vSUC x ∈ A
-`;
-
-val Inductives_def = Define`
-  Inductives = SPEC0 (λA. {} ∈ A ∧ ∀x. x ∈ A ⇒ vSUC x ∈ A)
-`;
-
-val inductive_Inductives = store_thm(
-  "inductive_Inductives",
-  ``inductive A ⇔ A ∈ Inductives``,
-  srw_tac [][inductive_def, Inductives_def, SPEC0]);
-
-val Nats_def = Define`
-  Nats = SPEC0 (λn. ∀s. inductive s ⇒ n ∈ s)
-`;
-
-val EMPTY_IN_Nats = store_thm(
-  "EMPTY_IN_Nats",
-  ``{} ∈ Nats``,
-  rw [Nats_def, SPEC0, inductive_def]);
-
-val vSUC_IN_Nats = store_thm(
-  "vSUC_IN_Nats",
-  ``n ∈ Nats ⇒ vSUC n ∈ Nats``,
-  rw [Nats_def, SPEC0, inductive_def, vSUC_def]);
-
-val SET_fromNat = store_thm(
-  "SET_fromNat",
-  ``SET (fromNat n)``,
-  Induct_on `n` >> srw_tac [][fromNat_def, vSUC_def]);
-val _ = export_rewrites ["SET_fromNat"]
-
-val fromNat_in_Nats = store_thm(
-  "fromNat_in_Nats",
-  ``∀n. fromNat n ∈ Nats``,
-  Induct THEN SRW_TAC [][fromNat_def] THENL [
-    SRW_TAC [][Nats_def, SPEC0] THEN
-    fs [inductive_def],
-    fs [Nats_def, SPEC0, vSUC_def] >>
-    fs [inductive_def, vSUC_def]
-  ]);
-val _ = export_rewrites ["fromNat_in_Nats"]
-
-val NOT_IN_0 = store_thm(
-  "NOT_IN_0",
-  ``x ∉ 0``,
-  SRW_TAC [][fromNat_def]);
-val _ = export_rewrites ["NOT_IN_0"]
-
-val vSUC_NOT_0 = store_thm(
-  "vSUC_NOT_0",
-  ``vSUC n ≠ 0``,
-  SRW_TAC [][vSUC_def, EXTENSION] THEN
-  Cases_on `n = 0` THEN SRW_TAC [][] THENL [
-    Q.EXISTS_TAC `0` THEN SRW_TAC [][],
-    METIS_TAC [fromNat_def, EMPTY_UNIQUE]
-  ]);
-val _ = export_rewrites ["vSUC_NOT_0"]
-
-val Nats_SET = store_thm(
-  "Nats_SET",
-  ``SET Nats``,
-  match_mp_tac SUBSETS_ARE_SETS >>
-  strip_assume_tac INFINITY >>
-  qexists_tac `w` >> simp [SUBSET_def] >>
-  qx_gen_tac `n` >> rw [Nats_def, SPEC0] >>
-  first_assum match_mp_tac >> simp [inductive_def] >> conj_tac
-    >- metis_tac [EMPTY_UNIQUE] >>
-  qx_gen_tac `e` >> strip_tac >>
-  `∃y. y ∈ w ∧ ∀u. u ∈ y ⇔ u ∈ e ∨ (u = e)` by metis_tac[] >>
-  qsuff_tac `vSUC e = y` >- rw[] >>
-  rw [vSUC_def, Once EXTENSION] >> metis_tac [SET_def]);
-
-val Nats_inductive = store_thm(
-  "Nats_inductive",
-  ``Nats ∈ Inductives``,
-  rw [SPEC0, SUBSET_def, Inductives_def, Nats_SET, EMPTY_IN_Nats,
-      vSUC_IN_Nats]);
-
-val Nats_least_inductive = store_thm(
-  "Nats_least_inductive",
-  ``P ∈ Inductives ⇒ Nats ⊆ P``,
-  rw[Inductives_def, SPEC0, SUBSET_def] >>
-  fs [Nats_def, SPEC0, inductive_def])
-
-val Nats_SETs = prove(``n ∈ Nats ⇒ SET n``, metis_tac [SET_def])
-val _ = augment_srw_ss [rewrites [Nats_SETs]]
-(*
-Higher order logic wins here: can capture all possible predicates.
-Can simplify to membership of a set S by making the predicate P be just that.
- ⊢ ∀P. P {} ∧ (∀x. P x ∧ x ∈ Nats ⇒ P (vSUC x)) ⇒ ∀u. u ∈ Nats ⇒ P u
-*)
-val nat_induction = save_thm(
-  "nat_induction",
-  Nats_least_inductive
-      |> SIMP_RULE(srw_ss())[SUBSET_def,Inductives_def,SPEC0]
-      |> Q.GEN `P`
-      |> Q.SPEC `SPEC0 P ∩ Nats`
-      |> SIMP_RULE (srw_ss() ++ CONJ_ss)
-                   [Nats_SET, EMPTY_IN_Nats, vSUC_IN_Nats, SPEC0,
-                    GSYM fromNat_def]
-      |> Q.GEN `P`);
-
-val transitive_def = Define`
-  transitive X ⇔ ∀x. x ∈ X ⇒ x ⊆ X
-`;
-
-val transitive_ALT = store_thm(
-  "transitive_ALT",
-  ``transitive X ⇔ ∀x y. x ∈ y ∧ y ∈ X ⇒ x ∈ X``,
-  rw [transitive_def] >> metis_tac [SUBSET_def]);
-
-val Nats_transitive = store_thm(
-  "Nats_transitive",
-  ``∀n. n ∈ Nats ⇒ transitive n``,
-  ho_match_mp_tac nat_induction >> conj_tac >> rw[transitive_def] >>
-  fs [vSUC_def, SUBSET_def] >> metis_tac []);
-
-val Nats_not_selfmembers = store_thm(
-  "Nats_not_selfmembers",
-  ``∀n. n ∈ Nats ⇒ n ∉ n``,
-  ho_match_mp_tac nat_induction >> rw[vSUC_def] >| [
-    strip_tac >> `n ∈ n ∪ {n}` by rw[] >>
-    metis_tac [Nats_transitive, transitive_ALT],
-    rw[Once EXTENSION] >> metis_tac []
-  ]);
-
-val pre_IN_vSUC = store_thm(
-  "pre_IN_vSUC",
-  ``SET n ⇒ n ∈ vSUC n``,
-  rw[vSUC_def]);
-
-val SET_vSUC = store_thm(
-  "SET_vSUC",
-  ``SET (vSUC n) = SET n``,
-  rw[vSUC_def, EQ_IMP_THM]);
-val _ = export_rewrites ["SET_vSUC"]
-
-val vSUC_11 = store_thm(
-  "vSUC_11",
-  ``∀n m. n ∈ Nats ∧ m ∈ Nats ⇒ ((vSUC n = vSUC m) ⇔ (n = m))``,
-  rw[EQ_IMP_THM] >>
-  `n ∈ vSUC m` by metis_tac [pre_IN_vSUC, SET_vSUC, Nats_SETs] >>
-  pop_assum mp_tac >> rw[vSUC_def] >>
-  `m ∈ vSUC n` by metis_tac [pre_IN_vSUC, SET_vSUC, Nats_SETs] >>
-  fs[vSUC_def] >>
-  metis_tac [transitive_ALT, Nats_transitive, Nats_not_selfmembers]);
-val _ = export_rewrites ["vSUC_11"]
-
 
 (*
 val FORMATION = new_axiom(
 
 *)
+
+val FOUNDATION = new_axiom(
+  "FOUNDATION",
+  ``(∀a. SET a ∧ a ⊆ w ⇒ a ∈ w) ⇒ ∀a. SET a ⇒ a ∈ w``);
+
+val IN_INDUCTION = store_thm(
+  "IN_INDUCTION",
+  ``(∀a. SET a ∧ (∀x. x ∈ a ⇒ P x) ⇒ P a) ⇒ ∀a. SET a ⇒ P a``,
+  rpt strip_tac >>
+  MP_TAC (INST [``w:vbgc`` |-> ``SPEC0 (λx. P x)``] FOUNDATION) >>
+  rw[SUBSET_def]);
+val _ = IndDefLib.export_rule_induction "IN_INDUCTION"
+
+val IN_REFL = store_thm(
+  "IN_REFL",
+  ``x ∉ x``,
+  Cases_on `SET x` >| [
+    pop_assum mp_tac >> qid_spec_tac `x` >>
+    ho_match_mp_tac IN_INDUCTION >> metis_tac [],
+    fs[SET_def]
+  ]);
+val _ = export_rewrites ["IN_REFL"]
+
+val IN_ANTISYM = store_thm(
+  "IN_ANTISYM",
+  ``x ∈ y ∧ y ∈ x ⇔ F``,
+  qsuff_tac `∀x. SET x ⇒ ∀y. y ∈ x ⇒ x ∉ y` >- metis_tac [SET_def] >>
+  Induct_on `SET x` >> metis_tac []);
 
 val _ = export_theory()
