examples/set-theory/vbg/vbgnatsScript.sml
@@ -1,0 +1,303 @@
+open HolKernel Parse boolLib bossLib
+open vbgsetTheory
+open lcsymtacs
+open boolSimps
+
+val _ = new_theory "vbgnats"
+
+val vSUC_def = Define`vSUC x = x ∪ {x}`
+
+val fromNat_def = Define`
+  (fromNat 0 = {}) ∧
+  (fromNat (SUC n) = vSUC (fromNat n))
+`;
+val _ = add_numeral_form(#"v", SOME "fromNat")
+
+val inductive_def = Define`
+  inductive A ⇔ SET A ∧ {} ∈ A ∧ ∀x. x ∈ A ⇒ vSUC x ∈ A
+`;
+
+val Inductives_def = Define`
+  Inductives = SPEC0 (λA. {} ∈ A ∧ ∀x. x ∈ A ⇒ vSUC x ∈ A)
+`;
+
+val inductive_Inductives = store_thm(
+  "inductive_Inductives",
+  ``inductive A ⇔ A ∈ Inductives``,
+  srw_tac [][inductive_def, Inductives_def, SPEC0]);
+
+val Nats_def = Define`
+  Nats = SPEC0 (λn. ∀s. inductive s ⇒ n ∈ s)
+`;
+
+val EMPTY_IN_Nats = store_thm(
+  "EMPTY_IN_Nats",
+  ``{} ∈ Nats``,
+  rw [Nats_def, SPEC0, inductive_def]);
+
+val vSUC_IN_Nats_I = store_thm(
+  "vSUC_IN_Nats_I",
+  ``n ∈ Nats ⇒ vSUC n ∈ Nats``,
+  rw [Nats_def, SPEC0, inductive_def, vSUC_def]);
+
+val SET_fromNat = store_thm(
+  "SET_fromNat",
+  ``SET (fromNat n)``,
+  Induct_on `n` >> srw_tac [][fromNat_def, vSUC_def]);
+val _ = export_rewrites ["SET_fromNat"]
+
+val fromNat_in_Nats = store_thm(
+  "fromNat_in_Nats",
+  ``∀n. fromNat n ∈ Nats``,
+  Induct THEN SRW_TAC [][fromNat_def] THENL [
+    SRW_TAC [][Nats_def, SPEC0] THEN
+    fs [inductive_def],
+    fs [Nats_def, SPEC0, vSUC_def] >>
+    fs [inductive_def, vSUC_def]
+  ]);
+val _ = export_rewrites ["fromNat_in_Nats"]
+
+val NOT_IN_0 = store_thm(
+  "NOT_IN_0",
+  ``x ∉ 0``,
+  SRW_TAC [][fromNat_def]);
+val _ = export_rewrites ["NOT_IN_0"]
+
+val vSUC_NOT_0 = store_thm(
+  "vSUC_NOT_0",
+  ``vSUC n ≠ 0``,
+  SRW_TAC [][vSUC_def, EXTENSION] THEN
+  Cases_on `n = 0` THEN SRW_TAC [][] THENL [
+    Q.EXISTS_TAC `0` THEN SRW_TAC [][],
+    METIS_TAC [fromNat_def, EMPTY_UNIQUE]
+  ]);
+val _ = export_rewrites ["vSUC_NOT_0"]
+
+val Nats_SET = store_thm(
+  "Nats_SET",
+  ``SET Nats``,
+  match_mp_tac SUBSETS_ARE_SETS >>
+  strip_assume_tac INFINITY >>
+  qexists_tac `w` >> simp [SUBSET_def] >>
+  qx_gen_tac `n` >> rw [Nats_def] >>
+  first_assum match_mp_tac >> simp [inductive_def] >> conj_tac
+    >- metis_tac [EMPTY_UNIQUE] >>
+  qx_gen_tac `e` >> strip_tac >>
+  `∃y. y ∈ w ∧ ∀u. u ∈ y ⇔ u ∈ e ∨ (u = e)` by metis_tac[] >>
+  qsuff_tac `vSUC e = y` >- rw[] >>
+  rw [vSUC_def, Once EXTENSION] >> metis_tac [SET_def]);
+
+val Nats_inductive = store_thm(
+  "Nats_inductive",
+  ``Nats ∈ Inductives``,
+  rw [SPEC0, SUBSET_def, Inductives_def, Nats_SET, EMPTY_IN_Nats,
+      vSUC_IN_Nats_I]);
+
+val Nats_least_inductive = store_thm(
+  "Nats_least_inductive",
+  ``P ∈ Inductives ⇒ Nats ⊆ P``,
+  rw[Inductives_def, SUBSET_def] >>
+  fs [Nats_def, inductive_def])
+
+val Nats_SETs = prove(``n ∈ Nats ⇒ SET n``, metis_tac [SET_def])
+val _ = augment_srw_ss [rewrites [Nats_SETs]]
+(*
+Higher order logic wins here: can capture all possible predicates.
+Can simplify to membership of a set S by making the predicate P be just that.
+ ⊢ ∀P. P 0 ∧ (∀x. P x ∧ x ∈ Nats ⇒ P (vSUC x)) ⇒ ∀u. u ∈ Nats ⇒ P u
+*)
+val nat_induction = save_thm(
+  "nat_induction",
+  Nats_least_inductive
+      |> SIMP_RULE(srw_ss())[SUBSET_def,Inductives_def,SPEC0]
+      |> Q.GEN `P`
+      |> Q.SPEC `SPEC0 P ∩ Nats`
+      |> SIMP_RULE (srw_ss() ++ CONJ_ss)
+                   [Nats_SET, EMPTY_IN_Nats, vSUC_IN_Nats_I,
+                    GSYM fromNat_def]
+      |> Q.GEN `P`);
+val _ = IndDefLib.export_rule_induction "nat_induction"
+
+val transitive_def = Define`
+  transitive X ⇔ ∀x. x ∈ X ⇒ x ⊆ X
+`;
+
+val transitive_ALT = store_thm(
+  "transitive_ALT",
+  ``transitive X ⇔ ∀x y. x ∈ y ∧ y ∈ X ⇒ x ∈ X``,
+  rw [transitive_def] >> metis_tac [SUBSET_def]);
+
+val Nats_transitive = store_thm(
+  "Nats_transitive",
+  ``∀n. n ∈ Nats ⇒ transitive n``,
+  ho_match_mp_tac nat_induction >> conj_tac >> rw[transitive_def] >>
+  fs [vSUC_def, SUBSET_def] >> metis_tac []);
+
+(* pointless given axiom of foundation - in its absence, this proof works
+val Nats_not_selfmembers = store_thm(
+  "Nats_not_selfmembers",
+  ``∀n. n ∈ Nats ⇒ n ∉ n``,
+  ho_match_mp_tac nat_induction >> rw[vSUC_def] >| [
+    strip_tac >> `n ∈ n ∪ {n}` by rw[] >>
+    metis_tac [Nats_transitive, transitive_ALT],
+    rw[Once EXTENSION] >> metis_tac []
+  ]);
+*)
+
+val pre_IN_vSUC = store_thm(
+  "pre_IN_vSUC",
+  ``SET n ⇒ n ∈ vSUC n``,
+  rw[vSUC_def]);
+
+val SET_vSUC = store_thm(
+  "SET_vSUC",
+  ``SET (vSUC n) = SET n``,
+  rw[vSUC_def, EQ_IMP_THM]);
+val _ = export_rewrites ["SET_vSUC"]
+
+(* doing this the longwinded way, with appeals to foundation all over the
+   place gives a stronger rewrite rule without requiring n and m to be ∈ Nats *)
+val vSUC_11 = store_thm(
+  "vSUC_11",
+  ``∀n m. ((vSUC n = vSUC m) ⇔ (n = m))``,
+  rw[EQ_IMP_THM] >> Cases_on `SET n` >| [
+    fs[vSUC_def] >> rw[EXTENSION] >>
+    `SET m` by metis_tac [UNION_SET_CLOSED, SET_INSERT, EMPTY_SET] >>
+    first_assum (qspec_then `x` mp_tac o
+                 SIMP_RULE (srw_ss()) [Once EXTENSION]) >>
+    simp[] >>
+    Cases_on `x ∈ n` >> simp[] >| [
+      rw[DISJ_IMP_THM] >> strip_tac >> rw[] >>
+      first_assum (qspec_then `n` mp_tac o
+                   SIMP_RULE (srw_ss()) [Once EXTENSION]) >>
+      rw[] >> metis_tac [IN_ANTISYM, IN_REFL],
+      Cases_on `x = n` >> simp[DISJ_IMP_THM] >> strip_tac >> rw[] >>
+      first_assum (qspec_then `m` mp_tac o
+                   SIMP_RULE (srw_ss()) [Once EXTENSION]) >>
+      rw[] >> metis_tac [IN_ANTISYM, IN_REFL]
+    ],
+
+    fs[vSUC_def] >>
+    `¬SET m` by metis_tac [UNION_SET_CLOSED, SET_INSERT, EMPTY_SET] >>
+    `({n} = {}) ∧ ({m} = {})`
+       by metis_tac [INSERT_def, PCLASS_SINGC_EMPTY, EMPTY_UNION] >>
+    fs[]
+  ]);
+val _ = export_rewrites ["vSUC_11"]
+
+val Nats_CASES = store_thm(
+  "Nats_CASES",
+  ``∀n. n ∈ Nats ⇔ (n = 0) ∨ ∃m. m ∈ Nats ∧ (n = vSUC m)``,
+  simp_tac (srw_ss() ++ DNF_ss)[EQ_IMP_THM, vSUC_IN_Nats_I] >>
+  Induct_on `n ∈ Nats` >> metis_tac []);
+
+val vSUC_IN_NATS = store_thm(
+  "vSUC_IN_NATS",
+  ``∀n. vSUC n ∈ Nats ⇔ n ∈ Nats``,
+  simp[EQ_IMP_THM, vSUC_IN_Nats_I] >>
+  qsuff_tac `∀m. m ∈ Nats ⇒ ∀n. (m = vSUC n) ⇒ n ∈ Nats` >- metis_tac [] >>
+  Induct_on `m ∈ Nats` >> simp[]);
+val _ = export_rewrites ["vSUC_IN_NATS"]
+
+(* less than or equal *)
+val nle_def = Define`
+  nle = SPEC0 (λp. ∀P. (∀x. x ∈ Nats ⇒ 〈0·x〉 ∈ P) ∧
+                       (∀x y. x ∈ Nats ∧ y ∈ Nats ∧ 〈x·y〉 ∈ P ⇒
+                              〈vSUC x·vSUC y〉 ∈ P) ⇒
+                       p ∈ P)
+`;
+
+val _ = overload_on ("<=", ``λx y. 〈x·y〉 ∈ nle``)
+
+val ZERO_LE = store_thm(
+  "ZERO_LE",
+  ``∀n. n ∈ Nats ⇒ 0 ≤ n``,
+  rw [nle_def]);
+val _ = export_rewrites ["ZERO_LE"]
+
+val nle_Nats = store_thm(
+  "nle_Nats",
+  ``n ≤ m ⇒ n ∈ Nats ∧ m ∈ Nats``,
+  rw[nle_def] >> pop_assum (qspec_then `Nats × Nats` mp_tac) >>
+  asm_simp_tac (srw_ss() ++ CONJ_ss)[CROSS_def]);
+
+val nle_induct = store_thm(
+  "nle_induct",
+  ``(∀n. n ∈ Nats ⇒ P 0 n) ∧
+    (∀n m. n ∈ Nats ∧ m ∈ Nats ∧ P n m ⇒ P (vSUC n) (vSUC m)) ⇒
+    ∀n m. n ≤ m ⇒ P n m``,
+  rw[nle_def] >>
+  qsuff_tac `〈n·m〉 ∈ SPEC0 (λp. ∃x y. (p = 〈x·y〉) ∧ P x y)` >-
+    simp_tac (srw_ss()) [] >>
+  pop_assum match_mp_tac >> simp[]);
+val _ = IndDefLib.export_rule_induction "nle_induct"
+
+val vSUC_LE_I = store_thm(
+  "vSUC_LE_I",
+  ``n ≤ m ⇒ vSUC n ≤ vSUC m``,
+  strip_tac >> imp_res_tac nle_Nats >>
+  fs[nle_def]);
+
+val LE_CASES = store_thm(
+  "LE_CASES",
+  ``n ≤ m ⇔ (n = 0) ∧ m ∈ Nats ∨
+            ∃n0 m0. n0 ∈ Nats ∧ m0 ∈ Nats ∧ (n = vSUC n0) ∧
+                    (m = vSUC m0) ∧ n0 ≤ m0``,
+  Tactical.REVERSE EQ_TAC >- (rw[] >> rw[vSUC_LE_I]) >>
+  map_every qid_spec_tac [`m`, `n`] >> ho_match_mp_tac nle_induct >>
+  srw_tac [CONJ_ss][vSUC_LE_I] >> rw[vSUC_LE_I]);
+
+val vSUC_LE1 = store_thm(
+  "vSUC_LE1",
+  ``vSUC n ≤ vSUC m ⇔ n ≤ m``,
+  eq_tac >-
+     (asm_simp_tac (srw_ss() ++ CONJ_ss)
+                   [SimpL ``(==>)``, Once LE_CASES] >> rw[]) >>
+  rw[vSUC_LE_I]);
+val _ = export_rewrites ["vSUC_LE1"]
+
+val vSUC_ZERO_LE = store_thm(
+  "vSUC_ZERO_LE",
+  ``¬ (vSUC n ≤ 0)``,
+  rw[Once LE_CASES]);
+val _ = export_rewrites ["vSUC_ZERO_LE"]
+
+val LE_REFL0 = prove(
+  ``∀n. n ∈ Nats ⇒ n ≤ n``,
+  ho_match_mp_tac nat_induction >> rw[vSUC_LE_I])
+
+val LE_REFL = store_thm(
+  "LE_REFL",
+  ``n ≤ n ⇔ n ∈ Nats``,
+  metis_tac [nle_Nats, LE_REFL0]);
+val _ = export_rewrites ["LE_REFL"]
+
+val LE_ANTISYM0 = prove(
+  ``∀n m. n ≤ m ⇒ m ≤ n ⇒ (m = n)``,
+  ho_match_mp_tac nle_induct >> simp[vSUC_LE1] >>
+  rw[Once LE_CASES]);
+
+val LE_ANTISYM = store_thm(
+  "LE_ANTISYM",
+  ``∀n m. n ≤ m ∧ m ≤ n ⇒ (m = n)``,
+  metis_tac [LE_ANTISYM0]);
+
+val LE_TRANS = store_thm(
+  "LE_TRANS",
+  ``∀x y z. x ≤ y ∧ y ≤ z ⇒ x ≤ z``,
+  qsuff_tac `∀x y. x ≤ y ⇒ ∀z. y ≤ z ⇒ x ≤ z` >- metis_tac [] >>
+  ho_match_mp_tac nle_induct >> rw[] >|[
+    `z ∈ Nats` by metis_tac [nle_Nats] >> rw[],
+    pop_assum mp_tac >>
+    asm_simp_tac (srw_ss() ++ CONJ_ss) [SimpL ``(==>)``, Once LE_CASES] >>
+    asm_simp_tac (srw_ss() ++ DNF_ss)[]
+  ]);
+
+val LE_TOTAL = store_thm(
+  "LE_TOTAL",
+  ``∀n m. n ∈ Nats ∧ m ∈ Nats ⇒ n ≤ m ∨ m ≤ n``,
+  qsuff_tac `∀n. n ∈ Nats ⇒ ∀m. m ∈ Nats ⇒ n ≤ m ∨ m ≤ n` >- metis_tac[] >>
+  ho_match_mp_tac nat_induction >> rw[] >>
+  qspec_then `m` mp_tac Nats_CASES >> rw[] >> rw[]);
+
+val _ = export_theory()
